typechecking in Handshake.fst

src/tls/Epochs.fst
@@ -1,8 +1,8 @@
 module Epochs
 
 (* 
-    This modules implements the mutable state for the successive epochs allocated by KeySchedule and used by TLS. 
-    Its separation from Handshake and coding are somewhat arbitrary.
+    This modules implements the mutable state for the successive StAE epochs allocated by KeySchedule and used by TLS. 
+    Its separation from Handshake and coding is somewhat arbitrary.
     An elaboration would ensure that keys in old epochs are erased. 
     (i.e. we only keep old epoch AE logs for specifying authentication)
 *)
@@ -20,16 +20,16 @@ open TLSError
 open TLSInfo
 open TLSConstants
 open Range
-open HandshakeMessages
+//open HandshakeMessages
 open StAE
-open Negotiation
+//open Negotiation
 
 module HH = FStar.HyperHeap
 module HS = FStar.HyperStack
 module MR = FStar.Monotonic.RRef
 module MS = FStar.Monotonic.Seq
+type random = TLSInfo.random 
 
-// relocate?
 
 type epoch_region_inv (#i:id) (hs_rgn:rgn) (r:reader (peerId i)) (w:writer i) =
   disjoint hs_rgn (region w) /\
@@ -46,19 +46,16 @@ type epoch_region_inv (#i:id) (hs_rgn:rgn) (r:reader (peerId i)) (w:writer i) =
   //except for the hs_rgn, of course
   is_hs_rgn hs_rgn
 
-abstract
-type epoch_region_inv'
+abstract type epoch_region_inv'
   (#i:id)
   (hs_rgn:rgn)
   (r:reader (peerId i))
   (w:writer i)
 = epoch_region_inv hs_rgn r w
 
-module I = IdNonce
-
-noeq type epoch (hs_rgn:rgn) (n:TLSInfo.random) =
+noeq type epoch (hs_rgn:rgn) (n:random) =
   | Epoch: #i:id{nonce_of_id i = n} ->
-      h:handshake ->
+      h:Negotiation.handshake ->
       r: reader (peerId i) ->
       w: writer i {epoch_region_inv' hs_rgn r w} -> epoch hs_rgn n
 // we would extend/adapt it for TLS 1.3,
@@ -71,24 +68,28 @@ let reveal_epoch_region_inv_all (u:unit)
   : Lemma (forall i hs_rgn r w.{:pattern (epoch_region_inv' #i hs_rgn r w)}
        epoch_region_inv' #i hs_rgn r w   <==>
        epoch_region_inv #i hs_rgn r w)
-  = ()
+=
+  ()
 
-let reveal_epoch_region_inv (#hs_rgn:rgn) (#n:TLSInfo.random) (e:epoch hs_rgn n)
+let reveal_epoch_region_inv (#hs_rgn:rgn) (#n:random) (e:epoch hs_rgn n)
   : Lemma (let r = Epoch?.r e in
        let w = Epoch?.w e in
        epoch_region_inv hs_rgn r w)
-  = ()
+= 
+  ()
 
-let writer_epoch (#hs_rgn:rgn) (#n:TLSInfo.random) (e:epoch hs_rgn n)
+let writer_epoch (#hs_rgn:rgn) (#n:random) (e:epoch hs_rgn n)
   : Tot (w:writer (e.i) {epoch_region_inv hs_rgn (Epoch?.r e) w})
-  = Epoch?.w e
+= 
+  Epoch?.w e
 
-let reader_epoch (#hs_rgn:rgn) (#n:TLSInfo.random) (e:epoch hs_rgn n)
+let reader_epoch (#hs_rgn:rgn) (#n:random) (e:epoch hs_rgn n)
   : Tot (r:reader (peerId e.i) {epoch_region_inv hs_rgn r (Epoch?.w e)})
-  = Epoch?.r e
+= 
+  Epoch?.r e
 
 (* The footprint just includes the writer regions *)
-let epochs_inv (#r:rgn) (#n:TLSInfo.random) (es: seq (epoch r n)) =
+let epochs_inv (#r:rgn) (#n:random) (es: seq (epoch r n)) =
   forall (i:nat { i < Seq.length es })
     (j:nat { j < Seq.length es /\ i <> j}).{:pattern (Seq.index es i); (Seq.index es j)}
     let ei = Seq.index es i in
@@ -98,11 +99,10 @@ let epochs_inv (#r:rgn) (#n:TLSInfo.random) (es: seq (epoch r n)) =
     // each epoch writer lives in a region disjoint from the others
     disjoint (region ei.w) (region ej.w)
 
-abstract let epochs_inv' (#r:rgn) (#n:TLSInfo.random) (es: seq (epoch r n)) =
-  epochs_inv es
+abstract let epochs_inv' (#r:rgn) (#n:random) (es: seq (epoch r n)) = epochs_inv es
 
 let reveal_epochs_inv' (u:unit)
-  : Lemma (forall (r:rgn) (#n:TLSInfo.random) (es:seq (epoch r n)). {:pattern (epochs_inv' es)}
+  : Lemma (forall (r:rgn) (#n:random) (es:seq (epoch r n)). {:pattern (epochs_inv' es)}
          epochs_inv' es
          <==>
          epochs_inv es)
@@ -119,27 +119,25 @@ type epoch_ctr (#a:Type0) (#p:(seq a -> Type)) (r:rid) (es:MS.i_seq r a p) =
 // we keep a sequence of allocated epochs, 
 // together with counters for reading and writing
 //NS: probably need some anti-aliasing invariant of these three references
-noeq type epochs (r:rgn) (n:TLSInfo.random) = | MkEpochs: 
+noeq type epochs (r:rgn) (n:random) = | MkEpochs: 
   es: MS.i_seq r (epoch r n) (epochs_inv #r #n) ->
   read: epoch_ctr r es ->
   write: epoch_ctr r es -> epochs r n
 
-let containsT (#r:rgn) (#n:TLSInfo.random) (es:epochs r n) (h:mem) =
+let containsT (#r:rgn) (#n:random) (es:epochs r n) (h:mem) =
     MS.i_contains (MkEpochs?.es es) h 
 
 val alloc_log_and_ctrs: #a:Type0 -> #p:(seq a -> Type0) -> r:rgn ->
-  ST (is:MS.i_seq r a p &
-      c1:epoch_ctr r is &
-      c2:epoch_ctr r is)
-     (requires (fun h -> p Seq.createEmpty))
-     (ensures (fun h0 x h1 ->
-       modifies_one r h0 h1
-       /\ modifies_rref r !{} (HS.HS?.h h0) (HS.HS?.h h1)
-       /\ (let (| is, c1, c2 |) = x in
-      i_contains is h1
-      /\ m_contains c1 h1
-      /\ m_contains c2 h1
-      /\ i_sel h1 is == Seq.createEmpty)))
+  ST (is:MS.i_seq r a p & c1:epoch_ctr r is & c2:epoch_ctr r is)
+    (requires (fun h -> p Seq.createEmpty))
+    (ensures (fun h0 x h1 ->
+      modifies_one r h0 h1 /\ 
+      modifies_rref r !{} (HS.HS?.h h0) (HS.HS?.h h1) /\ 
+      (let (| is, c1, c2 |) = x in
+      i_contains is h1 /\
+      m_contains c1 h1 /\
+      m_contains c2 h1 /\ 
+      i_sel h1 is == Seq.createEmpty)))
 let alloc_log_and_ctrs #a #p r =
   let init = Seq.createEmpty in
   let is = alloc_mref_iseq p r init in
@@ -148,15 +146,19 @@ let alloc_log_and_ctrs #a #p r =
   let c2 : epoch_ctr #a #p r is = m_alloc r (-1) in
   (| is, c1, c2 |)
 
-val incr_epoch_ctr: #a:Type0 -> #p:(seq a -> Type0) -> #r:rgn -> #is:MS.i_seq r a p
-          -> ctr:epoch_ctr r is
-          -> ST unit
-   (requires (fun h -> 1 + m_sel h ctr < Seq.length (i_sel h is)))
-   (ensures (fun h0 _ h1 ->
-                  let ctr_as_hsref = MR.as_hsref ctr in
-          modifies_one r h0 h1
-          /\ modifies_rref r !{as_ref ctr_as_hsref} (HS.HS?.h h0) (HS.HS?.h h1)
-          /\ m_sel h1 ctr = m_sel h0 ctr + 1))
+val incr_epoch_ctr :
+  #a:Type0 ->
+  #p:(seq a -> Type0) ->
+  #r:rgn ->
+  #is:MS.i_seq r a p ->
+  ctr:epoch_ctr r is ->
+  ST unit
+    (requires fun h -> 1 + m_sel h ctr < Seq.length (i_sel h is))
+    (ensures (fun h0 _ h1 ->
+      let ctr_as_hsref = MR.as_hsref ctr in
+      modifies_one r h0 h1 /\
+      modifies_rref r !{as_ref ctr_as_hsref} (HS.HS?.h h0) (HS.HS?.h h1) /\
+      m_sel h1 ctr = m_sel h0 ctr + 1))
 let incr_epoch_ctr #a #p #r #is ctr =
   m_recall ctr;
   let cur = m_read ctr in
@@ -164,10 +166,10 @@ let incr_epoch_ctr #a #p #r #is ctr =
   witness is (int_at_most (cur + 1) is);
   m_write ctr (cur + 1)
        
-val create: r:rgn -> n:TLSInfo.random -> ST (epochs r n)
-       (requires (fun h -> True))
-       (ensures (fun h0 x h1 -> modifies_one r h0 h1 /\ modifies_rref r !{} (HS.HS?.h h0) (HS.HS?.h h1)))
-let create (r:rgn) (n:TLSInfo.random) =
+val create: r:rgn -> n:random -> ST (epochs r n)
+    (requires (fun h -> True))
+    (ensures (fun h0 x h1 -> modifies_one r h0 h1 /\ modifies_rref r !{} (HS.HS?.h h0) (HS.HS?.h h1)))
+let create (r:rgn) (n:random) =
   let (| esref, c1, c2 |) = alloc_log_and_ctrs #(epoch r n) #(epochs_inv #r #n) r in
   MkEpochs esref c1 c2
 
@@ -181,33 +183,32 @@ unfold let incr_post #r #n (es:epochs r n) (proj:(es:epochs r n -> Tot (epoch_ct
   let oldr = m_sel h0 ctr in
   let newr = m_sel h1 ctr in
   let ctr_as_hsref = MR.as_hsref ctr in
-  modifies_one r h0 h1
-  /\ HH.modifies_rref r !{HH.as_ref (MkRef?.ref ctr_as_hsref)} (HS.HS?.h h0) (HS.HS?.h h1)
-  /\ newr = oldr + 1
+  modifies_one r h0 h1 /\
+  HH.modifies_rref r !{HH.as_ref (MkRef?.ref ctr_as_hsref)} (HS.HS?.h h0) (HS.HS?.h h1) /\ 
+  newr = oldr + 1
 
-val add_epoch: #r:rgn -> #n:TLSInfo.random ->
-               es:epochs r n -> e: epoch r n -> ST unit
-       (requires (fun h -> 
-       let is = MkEpochs?.es es in
-       epochs_inv #r #n (Seq.snoc (i_sel h is) e)))
-       (ensures (fun h0 x h1 -> 
-           let es = MkEpochs?.es es in
-           let es_as_hsref = MR.as_hsref es in
-            modifies_one r h0 h1  
-            /\ modifies_rref r !{as_ref es_as_hsref} (HS.HS?.h h0) (HS.HS?.h h1)
-            /\ i_sel h1 es == Seq.snoc (i_sel h0 es) e))
-let add_epoch #r #n (MkEpochs es _ _) e = 
-    MS.i_write_at_end es e
+val add_epoch :
+  #r:rgn -> #n:random -> es:epochs r n -> e:epoch r n ->
+  ST unit
+    (requires fun h -> let is = MkEpochs?.es es in epochs_inv #r #n (Seq.snoc (i_sel h is) e))
+    (ensures fun h0 x h1 ->
+        let es = MkEpochs?.es es in
+        let es_as_hsref = MR.as_hsref es in
+        modifies_one r h0 h1 /\ modifies_rref r !{as_ref es_as_hsref} (HS.HS?.h h0) (HS.HS?.h h1) /\
+        i_sel h1 es == Seq.snoc (i_sel h0 es) e)
+let add_epoch #r #n (MkEpochs es _ _) e = MS.i_write_at_end es e
 
 let incr_reader #r #n (es:epochs r n) : ST unit
     (requires (incr_pre es MkEpochs?.read))
     (ensures (incr_post es MkEpochs?.read))
-    = incr_epoch_ctr (MkEpochs?.read es)
+= 
+  incr_epoch_ctr (MkEpochs?.read es)
 
 let incr_writer #r #n (es:epochs r n) : ST unit
     (requires (incr_pre es MkEpochs?.write))
     (ensures (incr_post es MkEpochs?.write))
-    = incr_epoch_ctr (MkEpochs?.write es)
+= 
+  incr_epoch_ctr (MkEpochs?.write es)
 
 let get_epochs #r #n (es:epochs r n) = MkEpochs?.es es
 
@@ -215,33 +216,37 @@ let ctr (#r:_) (#n:_) (e:epochs r n) (rw:rw) = match rw with
   | Reader -> e.read
   | Writer -> e.write
 
-val readerT: #rid:rgn -> #n:TLSInfo.random -> e:epochs rid n -> mem -> GTot (epoch_ctr_inv rid (get_epochs e))
+val readerT: #rid:rgn -> #n:random -> e:epochs rid n -> mem -> GTot (epoch_ctr_inv rid (get_epochs e))
 let readerT #rid #n (MkEpochs es r w) (h:mem) = m_sel h r
 
-val writerT: #rid:rgn -> #n:TLSInfo.random -> e:epochs rid n -> mem -> GTot (epoch_ctr_inv rid (get_epochs e))
+val writerT: #rid:rgn -> #n:random -> e:epochs rid n -> mem -> GTot (epoch_ctr_inv rid (get_epochs e))
 let writerT #rid #n (MkEpochs es r w) (h:mem) = m_sel h w
 
-unfold let get_ctr_post (#r:rgn) (#n:TLSInfo.random) (es:epochs r n) (rw:rw) h0 (i:int) h1 = 
+unfold let get_ctr_post (#r:rgn) (#n:random) (es:epochs r n) (rw:rw) h0 (i:int) h1 = 
   let epochs = MkEpochs?.es es in
-  h0 == h1
-  /\ i = m_sel h1 (ctr es rw)
-  /\ -1 <= i
-  /\ MS.int_at_most i epochs h1
+  h0 == h1 /\ 
+  i = m_sel h1 (ctr es rw) /\ 
+  -1 <= i /\ 
+  MS.int_at_most i epochs h1
 
-let get_ctr (#r:rgn) (#n:TLSInfo.random) (es:epochs r n) (rw:rw)
-  : ST int (requires (fun h -> True))
-         (ensures (get_ctr_post es rw))
-  = let epochs = es.es in
-    let n = m_read (ctr es rw) in
-    testify (MS.int_at_most n epochs);
-    n      
+let get_ctr (#r:rgn) (#n:random) (es:epochs r n) (rw:rw)
+  : ST int (requires (fun h -> True)) (ensures (get_ctr_post es rw))
+= 
+  let epochs = es.es in
+  let n = m_read (ctr es rw) in
+  testify (MS.int_at_most n epochs);
+  n      
 
-let get_reader (#r:rgn) (#n:TLSInfo.random) (es:epochs r n) = get_ctr es Reader
-let get_writer (#r:rgn) (#n:TLSInfo.random) (es:epochs r n) = get_ctr es Writer
+let get_reader (#r:rgn) (#n:random) (es:epochs r n) = get_ctr es Reader
+let get_writer (#r:rgn) (#n:random) (es:epochs r n) = get_ctr es Writer
 
 let epochsT #r #n (es:epochs r n) (h:mem) = MS.i_sel h (MkEpochs?.es es)
-  
-let get_current_epoch (#r:_) (#n:_) (e:epochs r n) (rw:rw)
+
+let get_current_epoch
+  (#r:_)
+  (#n:_)
+  (e:epochs r n)
+  (rw:rw)
   : ST (epoch r n)
        (requires (fun h -> 0 <= m_sel h (ctr e rw)))
        (ensures (fun h0 rd h1 -> 
@@ -250,14 +255,12 @@ let get_current_epoch (#r:_) (#n:_) (e:epochs r n) (rw:rw)
            h0==h1 /\
            Seq.indexable epochs j /\
            rd == Seq.index epochs j))
-  = let j = get_ctr e rw in 
-    let epochs = MS.i_read e.es in
-    Seq.index epochs j
+= 
+  let j = get_ctr e rw in 
+  let epochs = MS.i_read e.es in
+  Seq.index epochs j
 
-
-val recordInstanceToEpoch: #r:rgn -> #n:TLSInfo.random ->
-  hs:Negotiation.handshake ->
-  ks:KeySchedule.recordInstance -> 
-  Tot (epoch r n)
-let recordInstanceToEpoch #hs_rgn #n hs (KeySchedule.StAEInstance #i rd wr) =
-  Epoch hs rd wr
+val recordInstanceToEpoch: 
+  #r:rgn -> #n:random -> hs:Negotiation.handshake -> 
+  ks:KeySchedule.recordInstance -> Tot (epoch r n)
+let recordInstanceToEpoch #hs_rgn #n hs (KeySchedule.StAEInstance #i rd wr) = Epoch hs rd wr
